Messed around with eltype to use ordinals ssreflect, still in progress, saving

scrap.v
@@ -1,6 +1,262 @@
+Set Warnings "-notation-overridden,-parsing".
+From Coq Require Import Bool.Bool Init.Nat Arith.Arith Arith.EqNat
+     Init.Datatypes Lists.List Strings.String Program Sumbool.
+Require Export Coq.Strings.String.
+From mathcomp Require Import ssrnat ssreflect ssrfun ssrbool eqtype fintype.
+From Semantics Require Import lemmas_0.
+
+(*basic list functions that I couldn't find in a library*)
+Open Scope list_scope.
+Fixpoint eq_lists {A: Type} (L1: list A) (L2: list A) (eq: A -> A -> Prop) :=
+        match L1, L2 with
+          nil, nil => True
+        | (w::ws), (d::ds) => (eq w d) /\ (eq_lists ws ds eq) (*considers order*)
+        | _ , _ => False end.
+
+Fixpoint member {A: Type} (eq: A -> A -> bool) (a: A)  (L: list A) :=
+  match L with
+    [] => false
+  | x::xs => orb (eq a x) (member eq a xs)
+  end.
+
+Definition intersect := forall {A: Type} (L1 L2: list A),
+    exists(x: A), ((In x L1) /\ (In x L2)).
+
+Definition prefix {A: Type} (O1: list A) (O2: list A) :=
+  exists(l: nat), O1 = firstn l O2.
+
+Check intersect.
+Check prefix.
+
+Definition bar := forall n: nat, n= 0.
+Definition foo := fun n: nat => n = 0.
+
+
+Fixpoint loop (n: nat) : unit := let _ := (loop n) in tt.
+
+Compute (loop 0).
+
+(*Eval cbv in (loop 0).*)
+
+Print loop.
+
+(*Goal forall n : nat, (fix loop (n: nat) := n) n = n.
+  intros n.
+  destruct n.
+  reflexivity. Qed.*)
+
+(*Goal forall n : nat, (fun x=> x) n = n.
+  reflexivity.
+
+Goal (fun x => x) 42 = 42.
+  reflexivity.
+
+Goal bar = forall n: nat, foo n.
+  reflexivity.
+  unfold foo. reflexivity.*)
+
+
+Close Scope list_scope.
+
+Open Scope string_scope.
+(*---*)
+
+
+(*setting up strings equality type*)
+(* eqb_string and
+eqb_string_true_iff taken from software foundations*)
+Definition eqb_string (x y : string) : bool :=
+  if string_dec x y then true else false.
+
+Lemma eqb_string_true_iff : forall x y : string,
+    eqb_string x y = true <-> x = y.
+Proof.
+   intros x y.
+   unfold eqb_string.
+   destruct (string_dec x y) as [H |Hs].
+   - subst. split. reflexivity. reflexivity.
+   - split.
+     + intros contra. discriminate contra.
+     + intros H. rewrite H in Hs *. destruct Hs. reflexivity.
+Qed.
+(*what is the star*)
+Lemma eqstring: Equality.axiom eqb_string.
+Proof.
+  unfold Equality.axiom. intros.
+  destruct (eqb_string x y) eqn:beq.
+  - constructor. apply eqb_string_true_iff in beq. assumption.
+  -  constructor. intros contra. apply eqb_string_true_iff in contra.
+     rewrite contra in beq. discriminate beq.
+Qed.
+Canonical string_eqMixin := EqMixin eqstring.
+Canonical string_eqtype := Eval hnf in EqType string string_eqMixin.
+(***)
+
+
+(*Now, to business! Below is syntax*)
+Open Scope type_scope.
+
+Inductive boptype :=
+  Plus
+| Sub
+| Mult
+| Div
+| Mod
+| Or
+| And.
+
+(*shortcut!*)
+Inductive value :=
+    Nat (n: nat)
+  | Bool (b: bool)
+  | error. 
+Coercion Bool : bool >-> value.
+Coercion Nat : nat >-> value.
+
+Definition eqb_value (x y: value) :=
+  match x, y with
+    Nat nx, Nat ny => nx == ny
+  | Bool bx, Bool byy => bx == byy
+  | error, error => true
+  | _, _ => false
+  end.
+
+Lemma eqb_value_true_iff : forall x y : value,
+    is_true(eqb_value x y) <-> x = y.
+Proof.
+  intros. destruct x, y; split; simpl; 
+            try (move/eqP ->); try (intros H; inversion H); auto.
+Qed.
+
+(*look in here!*)
+(*Lemma eqb_value_true_iff1 : forall x y : value,
+    is_true(eqb_value x y) <-> x = y.
+Proof.
+  intros. destruct x, y; split; simpl; try (intros H; discriminate H).
+  - move/eqP ->. reflexivity.
+  - by move => [->].
+  - move/eqP ->. reflexivity.
+  - intros H. inversion H. apply eq_refl.
+  - auto.
+  - auto.*)
+
+    (*move => []*)
+
+Lemma eqvalue: Equality.axiom eqb_value.
+Proof.
+  unfold Equality.axiom. intros.
+  destruct (eqb_value x y) eqn:beq.
+  - constructor. apply eqb_value_true_iff in beq. assumption.
+  -  constructor. intros contra. apply eqb_value_true_iff in contra.
+     rewrite contra in beq. discriminate beq.
+Qed.
+Canonical value_eqMixin := EqMixin eqvalue.
+Canonical value_eqtype := Eval hnf in EqType value value_eqMixin.
+
+(*evaluation rules for binary operations*)
+
+Fixpoint bopeval (bop: boptype) (v1 v2 :value): (value) :=
+  match bop with
+   Plus => 
+    (
+      match v1, v2 with
+        (Nat n1), (Nat n2) => Nat (add n1 n2)
+        | _, _ => error
+        end
+    )
+  | Sub => 
+    (
+      match v1, v2 with
+       (Nat n1), (Nat n2) => Nat (n1 - n2)
+        | _, _ => error
+        end
+    )
+  | Mult => 
+    (
+      match v1, v2 with
+       (Nat n1), (Nat n2) => Nat (mul n1 n2)
+        | _, _ => error
+        end
+    )
+  | Div =>
+    (
+      match v1, v2 with
+       (Nat n1), (Nat n2) =>
+                    ( if (n2 == 0) then error
+                      else Nat (n1 / n2))
+        | _, _ => error
+        end
+    )
+  | Mod =>
+    (
+      match v1, v2 with
+       (Nat n1), (Nat n2) =>
+                    ( if (n2 == 0) then error
+                     else Nat (n1 mod n2))
+        | _, _ => error
+        end
+    )
+  | Or =>
+  (
+      match v1, v2 with
+        (Bool b1), (Bool b2) => Bool (orb b1 b2)
+        | _, _ => error
+        end
+    )
+  | And =>
+  (
+      match v1, v2 with
+        (Bool b1), (Bool b2) => Bool (andb b1 b2)
+        | _, _ => error
+        end
+  )
+  end.
+
+(*value helper functions*)
+Definition isvaluable (v: value) :=
+  match v with
+    error => False
+  | _ => True
+  end.
+
+Definition isvalidbop (bop: boptype) (v1 v2 : value) :=
+  match (bopeval bop v1 v2) with
+    error => False
+  | _ => True
+  end.
+
+
+(*memory maps...used for both memories and checkpoints*)
+Definition map_t (A: eqType) := A -> value.
+
+(*memory helpers*)
+Definition emptymap A :(map_t A) := (fun _ => error).
+Definition updatemap {A} (m: map_t A) (i: A) (v: value) : map_t A := (fun j =>
+                                                               if (j ==i) then v
+                                                               else (m j)).
+Notation "i '|->' v ';' m" := (updatemap m i v)
+  (at level 100, v at next level, right associativity).
+(*in (m1 U! m2), m1 is checked first, then m2*)
+
+Definition indomain {A} (m: map_t A) (x: A) :=
+  match m x with
+    error => False
+  | _ => True
+  end.
+(*this function is NOT used to check the domain of checkpoint maps.
+ In particular, because an entire array can be checkpointed even if only
+ one element has been assigned to (while the other elements may, in theory, still be unassigned),
+(in particular, I refer to D-WAR-CP-Arr)
+this function would return that assigned array elements are in the domain of N, while the unassigned array
+elements are not, even though both have been checkpointed.
+ I resolved this problem by defining indomain_nvm, used for checkpoint maps in algorithms.v, which
+checks if a warvar is in the domain, rather than checking a location.
+ *)
+(******************************************************************************************)
+
+(*******************************more syntax**********************************************)
 Inductive array :=
   Array (s: string) (l: nat).
-
 
 Inductive volatility :=
   nonvol
@@ -10,13 +266,14 @@ Inductive smallvar :=
   SV (s: string) (q: volatility).
 
 Inductive dangerous_el :=
-  El_d (a: array) (n: nat).
+  El_d (a: array) (n: value).
 
 (*used subtypes to enforce the fact that only some expressions are
  memory locations*)
 Definition elpred  := (fun x=> match x with
-                                        El_d (Array _ length) i => (i <? length)
-                                 end).
+                                        El_d (Array _ length) (Nat i) => (i <? length)
+                            | _ => false                                            
+                            end).
 (*elpred checks if index is a natural in bounds*)
 
 Notation el := {x: dangerous_el | elpred x}.
@@ -40,155 +297,702 @@ Notation "a '[[' e ']]'" := (Element (a) (e))
 Definition loc := smallvar + el. (*memory location type*)
 
 Notation warvars := (list loc).
+(*Coercion (inl smallvar el): smallvar >-> loc.*)
+(*Coercion inl: smallvar >-> loc.*)
+
+(**location and warvar helper functions*)
+(**no need to work directly with the subtypes or sumtypes, just use these**)
+(**Note: some of these are currently unused due to implementation changes, but I left them
+ as they might be useful later*)
+
+(*array and el functions*)
+
+(*equality type for arrays*)
+Open Scope list_scope.
+Definition eqb_array (a1 a2: array) :=
+  match a1, a2 with
+    Array s1 l1, Array s2 l2 => andb (s1 == s2) (l1 == l2)
+  end.
+
+Lemma eqb_array_true_iff : forall x y : array,
+    is_true(eqb_array x y) <-> x = y.
+Proof.
+  intros. destruct x, y; split; simpl.
+  - move/(reflect_conj eqP eqP).
+    case => H0 H1. subst. reflexivity.
+  - intros H. inversion H.
+    apply (introT (reflect_conj eqP eqP)). (*ask arthur is there a
+                                            way to do this using ssreflect
+                                            rather than the introT
+                                            lemma*)
+    split; reflexivity.
+Qed.
+
+Lemma eqarray: Equality.axiom eqb_array.
+Proof.
+  unfold Equality.axiom. intros.
+  destruct (eqb_array x y) eqn:beq.
+  - constructor. apply eqb_array_true_iff in beq. assumption.
+  -  constructor. intros contra. apply eqb_array_true_iff in contra.
+     rewrite contra in beq. discriminate beq.
+Qed.
+Canonical array_eqMixin := EqMixin eqarray.
+Canonical array_eqtype := Eval hnf in EqType array array_eqMixin.
+(*****)
+
+(*equality type for elements*)
+
+Definition eqb_el_d (x y:dangerous_el) :=
+  match x, y with
+    El_d ax ix, El_d ay iy => (ax==ay) && (ix == iy) end.
 
 
-Inductive trace_c: context -> context -> obseq -> the_write_stuff -> Type :=
-  CTrace_Empty: forall(C: context),
-                 trace_c C C nil (nil, nil, nil)
-  | CTrace_Single: forall {C1 C2: context} {O: obseq} {W: the_write_stuff},
-      cceval_w C1 O C2 W ->
-      trace_c C1 C2 O W
-| CTrace_App: forall{C1 C2 Cmid: context} {O1 O2: obseq}
-               {W1 W2: the_write_stuff},
-    trace_c C1 Cmid O1 W1 -> (*steps first section*)
-    O1 <> [] -> (* forces empty step to use other constructors*)
-    O2 <> []  ->
-    trace_c Cmid C2 O2 W2 -> (*steps rest of program*)
-    trace_c C1 C2 (O1 ++ O2) (append_write W1 W2).
+Lemma eqb_eld_iff : forall x y : dangerous_el,
+    is_true(eqb_el_d x y) <-> x = y.
+Proof.
+  case => [ax ix] [ay yP]. simpl.
+  split. case / (reflect_conj eqP eqP) => [H1 H2]. by subst.
+  move => [H1 H2]. subst. apply/ (reflect_conj eqP eqP). auto.
+Qed.
 
-Program Definition trace_append {C1 Cmid C2: context }
-                  {O1 O2: obseq}
-                  {W1 W2: the_write_stuff}
-                  (T1: trace_c C1 Cmid O1 W1)
-                  (T2: trace_c Cmid C2 O2 W2) : trace_c C1 C2 (O1 ++ O2) (append_write W1 W2)
-  :=
-  match O1, O2 with
-    [], [] => T1 (*C1 = Cmid = C2*)
-  | [], _ => T2 (*C1 = Cmid*)
-  | _, [] => T1 (**)
-  | (x::xs), (y::ys) => CTrace_App T1 _ _ T2 end.
+Lemma eq_eld_iff: Equality.axiom eqb_el_d.
+Proof.
+  unfold Equality.axiom. intros.
+  destruct (eqb_el_d x y) eqn:beq.
+  - constructor. apply eqb_eld_iff in beq. assumption.
+  -  constructor. intros contra. apply eqb_eld_iff in contra.
+     rewrite contra in beq. discriminate beq.
+Qed.
+Check el.
+Check val.
+Check SubEqMixin.
+Check EqMixin.
+Check Equality.mixin_of.
+Canonical eld_eqMixin := EqMixin eq_eld_iff.
+Canonical eld_eqtype := Eval hnf in EqType dangerous_el eld_eqMixin.
+(*suggests it wants an equality relation for the big type before it lets
+ you have it for the subtype...that's annoying...ask arthur*)
+Check SubEqMixin.
+Check SubType.
 
-(*clean up this ltac*)
-Ltac empty T2 :=apply empty_trace in T2; [destruct T2 as [f g ]; inversion f; subst; try reflexivity |
-                                           reflexivity].
-Ltac empty2 T1 T2 := apply empty_trace in T1; [destruct T1 as [f g]; inversion g;
-                 subst; apply empty_trace in T2; [ destruct T2 as [h i]; inversion i;
-                 rewrite append_write_empty; reflexivity | reflexivity] | reflexivity].
+Definition testname := Array "a" 10.
+Definition testname1 := El_d testname 0.
+Lemma xworks: is_true (elpred testname1).
+  unfold elpred. unfold testname1. unfold testname. auto. Qed.
 
-Ltac emptyl T2 :=apply empty_trace in T2; [destruct T2 as [f g ]; inversion g; subst; try reflexivity |
-                                           reflexivity].
+Definition Test: el := eqtype.Sub testname1 xworks. (*ask arthur shouldn't coq be able to infer the subtype type*)
 
-Next Obligation. empty T2. Qed. 
-Next Obligation. empty2 T1 T2. Qed.           
-Next Obligation. empty T1. Qed.
-Next Obligation. emptyl T1. rewrite append_write_empty_l. reflexivity. Qed. 
-Next Obligation. empty T2. Qed.
-Next Obligation. symmetry. apply app_nil_r. Qed.
-Next Obligation. emptyl T2. rewrite append_write_empty. reflexivity. Qed.
-Next Obligation. split. intros wildcard contra. destruct contra. inversion H1.
-                 intros contra. destruct contra. inversion H1. Qed.
+Check Test == Test.
+
+(*smallvar functions*)
+Definition isNV_b (x: smallvar) := (*checks if x is stored in nonvolatile memory*)
+  match x with
+    SV _ nonvol => true
+  | _ => false
+  end.
+
+Definition isV_b (x: smallvar) :=(*checks if x is stored in volatile memory*)
+  match x with
+    SV _ vol => true
+  | _ => false
+  end.
+
+Definition isNV x := is_true(isNV_b x). (*prop version of isNV_b*)
+
+Definition isV x := is_true(isV_b x). (*prop version of isV_b*)
+
+Definition eqb_smallvar (x y: smallvar): bool :=
+  match x, y with
+    SV sx vol, SV sy vol => sx== sy
+  | SV sx nonvol, SV sy nonvol => sx== sy
+  | _, _ => false end.                                     
+
+Lemma eqb_smallvar_iff : forall x y : smallvar,
+    is_true(eqb_smallvar x y) <-> x = y.
+Proof.
+  intros. destruct x, y, q, q0; simpl;
+     try (split; [move/ eqP ->; reflexivity |
+                  intros H; inversion H; auto]);
+  try (split; [case => H; discriminate H | case => H H1; inversion H1]).
+Qed.
+
+Lemma eqsmallvar: Equality.axiom eqb_smallvar.
+Proof.
+  unfold Equality.axiom. intros.
+  destruct (eqb_smallvar x y) eqn:beq.
+  - constructor. apply eqb_smallvar_iff in beq. assumption.
+  -  constructor. intros contra. apply eqb_smallvar_iff in contra.
+     rewrite contra in beq. discriminate beq.
+Qed.
+
+Canonical smallvar_eqMixin := EqMixin eqsmallvar.
+Canonical smallvar_eqtype := Eval hnf in EqType smallvar smallvar_eqMixin.
+
+(*loc and warvar functions*)
+
+Definition eqb_loc (l1: loc) (l2: loc) :=
+  match l1, l2 with
+    inl x, inl y => x == y
+  | inr x, inr y => x == y
+  | _, _ => false 
+  end.
+
+(*equality type for locations*)
+
+Lemma eqb_loc_true_iff : forall x y : loc,
+    is_true(eqb_loc x y) <-> x = y.
+Proof.
+  case => [x1 | x2] [y1 | y2]; simpl; split; try (by move/ eqP ->);
+      try (by move => [] ->); intros H; inversion H.
+Qed.
+
+Lemma eqloc: Equality.axiom eqb_loc.
+Proof.
+  unfold Equality.axiom. intros.
+  destruct (eqb_loc x y) eqn:beq.
+  - constructor. apply eqb_loc_true_iff in beq. assumption.
+  -  constructor. intros contra. apply eqb_loc_true_iff in contra.
+     rewrite contra in beq. discriminate beq.
+Qed.
+Canonical loc_eqMixin := EqMixin eqloc.
+Canonical loc_eqtype := Eval hnf in EqType loc loc_eqMixin.
+
+Definition get_length (a: array) :=
+  match a with
+    Array _ length => length end.
+
+Definition index (a: array) := 'I_(get_length a).
+
+Definition generate_locs' (a: array): list (index a) := enum (index a).
+
+Check generate_locs'.
 
 
-(*intermittent traces*)
- (*the same as trace_c bar types as differences between
-  intermittent and continuous execution have been implemented in evals*)
-Inductive trace_i : iconf -> iconf -> obseq -> the_write_stuff -> Prop :=
-iTrace_Empty: forall{C: iconf},
-                 trace_i C C nil (nil, nil, nil)
-|iTrace_Single: forall{C1 C2: iconf} {O: obseq} {W: the_write_stuff},
-                  iceval_w C1 O C2 W -> (*command in C2 is skip by def single_com, iceval_w*)
-                  trace_i C1 C2 O W
-| iTrace_App: forall{C1 C2 Cmid: iconf} {O1 O2: obseq}
-         {W1 W2: the_write_stuff},
-    trace_i C1 Cmid O1 W1 -> (*steps first section*)
-    trace_i Cmid C2 O2 W2 -> (*steps rest of program*)
-    trace_i C1 C2 (O1 ++ O2) (append_write W1 W2).
-Definition multi_step_c (C1 C2: context) (O: obseq) :=
-    exists W: the_write_stuff, inhabited (trace_c C1 C2 O W).
-          
 
-Definition multi_step_i (C1 C2: iconf) (O: obseq) :=
-    exists W: the_write_stuff, trace_i C1 C2 O W.
-(*more trace helpers*)
+Sub (value) (proof)
 
-Definition Wt {C1 C2: context} {O: obseq} {W: the_write_stuff}
-  (T: trace_c C1 C2 O W) := getwt W.
+Check (enum _).
 
-Definition Rd {C1 C2: context} {O: obseq} {W: the_write_stuff}
-           (T: trace_c C1 C2 O W) := getrd W.
+Check enum [pred x: 'I_5 | x < 3 ]. 
 
-Definition FstWt {C1 C2: context} {O: obseq} {W: the_write_stuff}
-  (T: trace_c C1 C2 O W) := getfstwt W.
+Check [pred x: 'I_5 | x < 3 ].
+
+Check simpl_pred.
 
 
-(**********************************************************************************)
+Lemma annoying: forall(a: array) (n: nat),
+    (n < (get_length a)) -> is_true (elpred (El_d a (Nat n))).
+Admitted.
 
 
-(*relations between continuous and intermittent memory*)
+
+Fixpoint generate_locs (a: array) (n: nat) (H: (get_length a) < n) :=
+  match n with
+    0 => [Sub (El_d a (Nat 0)) (annoying H)]
+  | S n' => (Sub (El_d a (Nat n)) (annoying H))::
+                                              generate_locs a n'
+                                              (transitivity term)
+El_d a (Nat n)::(generate_locs a n') end.
+
+Definition array_to_el (a: array) :=
+  match a with
+    Array _ length => generate_locs a length end.
+
+Lemma elpredok: forall(a: array) (x: dangerous_el),
+    In x (array_to_el a) -> is_true (elpred x).
+Admitted.
+
+Definition array_to_loc (a: array) :=
+  map (fun x => el_to_loc (elpredok a) x ___)  (*how to communicate to map
+                                                  that the element it's manipulatin
+                                                  is in the argument list
+                                                  ask arthur*)
+
+(*******************************************************************)
+
+(*more syntax*)
+Inductive instruction :=
+  skip
+| asgn_sv (x: smallvar) (e: exp) (*could distinguish between NV and V assignments as well here*)
+| asgn_arr (a: array) (i: exp) (e: exp) (*i is index, e is new value of a[i]*)
+| incheckpoint (w: warvars)
+| inreboot.
+(*added the in prefixes to distinguish from the observation reboots
+ and checkpoints*)
+
+Inductive command :=
+  Ins (l: instruction)
+| Seqcom (l: instruction) (c: command) (*added suffix to distinguish from Seq ceval
+                                         constructor*)
+| ITE (e: exp) (c1: command) (c2: command).
+
+Notation "l ';;' c" := (Seqcom l c)
+                         (at level 100).
+
+Notation "'TEST' e 'THEN' c1 'ELSE' c2 " := (ITE e c1 c2)
+                                              (at level 100).
+Coercion Ins : instruction >-> command.
+
+(*******************************************************************)
+
+(******setting up location equality relation for memory maps******************)
+(****************************************************************)
+
+(****************************memory*************************************)
+
+(*memory locations defined above warvars*)
+Notation mem := (map_t loc_eqtype). (*memory mapping*)
+
+Inductive nvmem := (*nonvolatile memory*)
+  NonVol (m : mem) (D: warvars). (*extra argument to keep track of checkpointed warvars because
+                                  it might be nice to have for when we do checkpoint proofs*)
+
+Inductive vmem := (*volatile memory*)
+  Vol (m : mem).
+
+(*I could change nvmem and vmem to enforce that they only take in smallvars
+ of the correct type but it's already checked in my evaluation rules*)
+
+(**************************helpers for the memory maps*********************************************)
+
+(*note: a lot of these aren't being used right now because, after I changed the types
+ of DINO and WAR, they aren't necessary.
+ I won't delete them because having the domain of the checkpoint easily accessible and
+ manipulable could be handy in the future*)
+
+Definition getmap (N: nvmem) :=
+  match N with NonVol m _ => m end.
+
+Definition getdomain (N: nvmem) :=
+  match N with NonVol _ D => D end.
+
+Definition getvalue (N: nvmem) (i: loc) :=
+  (getmap N) i.
+  Notation "v '<-' N" := (getvalue N v)
+                           (at level 40).
 
 
-(*Definition 4*)
-(*concern: not yet clear to me why we need the vmem parameter; pending further inspection of
- proofs*)
-(*concern: liberal use of intensional equality with nvmem*)
-(*N0, V0 is starting state for both executions
- N1, V1 and Ncomp are middle states of intermittent, continuous respectively
- V1 isn't used anywhere it's just to fill out the type
- N2, V2 is final state for intermittent, once again solely to fill out the type*)
-Inductive same_pt: nvmem -> vmem -> command -> command -> nvmem -> nvmem -> Prop:=
-same_mem: forall {N0 N1 Ncomp N2: nvmem}
-                  {V0 V1 V2: vmem}
-                  {c0 c1 crem: command}
-                  {W1 W2: the_write_stuff}
-                  {w: warvars}
-                  {O1 O2: obseq}
-                  (T1: trace_c (N0, V0, c0) (N1, V1, c1) O1 W1)
-                  (T2: trace_c (N1, V1, c1) (N2, V2, ((incheckpoint w);; crem)) O2 W2),
-                  (getdomain N1) = (getdomain Ncomp) 
-                  -> not(In checkpoint O1)
-                  -> not (In checkpoint O2) (*checks checkpoint T2 ends on is nearest checkpoint*)
-                 -> (forall(l: loc),
-                      not((getmap N1) l = (getmap Ncomp) l)
-                      -> ((In l (getwt W2)) /\ (In l (getfstwt (append_write W1 W2))) /\ not (In l (getwt W1))))
-                  -> same_pt N0 V0 c0 c1 N1 Ncomp.
-(*Definition 5*)
-(*Nc0 is starting nvm for cont
-Ni0 is starting nvm for intermittent
- N1 V1 is middle state for intermittent
-N, V, c is checkpoint at middle state of intermittent
- Nend, Vend is final state for intermittent, not used, solely to fill out the type
- V1 isn't used anywhere it's just to fill out the type
- N2, V2 is final state for intermittent, once again solely to fill out the type*)
-Inductive current_init_pt: nvmem -> vmem -> command -> nvmem -> nvmem -> nvmem -> Prop:=
-  valid_mem: forall {N Ni0 N1 Nc0 Nend: nvmem}
-                  {V V1 Vend: vmem}
-                  {c crem: command}
-                  {W : the_write_stuff}
-                  {O: obseq}
-                  {w: warvars}
-                  (T: trace_c (Ni0, V, c) (Nend, Vend, (incheckpoint w);;crem) O W),
-                  (getdomain N1) = (getdomain Nc0) 
-                  -> not (In checkpoint O) (*checks checkpoint T ends on is nearest checkpoint*)
-                 -> (forall(l: loc),
-                      not((getmap N1) l = (getmap Nc0) l)
-                      -> (In l (getfstwt W)) \/ (In (loc_warvar l) (getdomain N)))
-                 -> current_init_pt N V c Ni0 N1 Nc0.
-(*Definition 6*)
-(*concern: Typo in paper, N0, V0 is left out of invocation of Def 4*)
-(*(N0, V0, c0) is checkpoint state at time c1
-N1 V c is intermittent state
-N2 V c is continuous state starting from same state as checkpoint
-concern: using context instead of cconf
+  (*updates domain and mapping function*)
+Definition updateNV (N: nvmem) (i: loc) (v: value) :=
+  match N with NonVol m D =>
+               NonVol (updatemap m i v) (i:: D)  end.
+
+(*used to update NV memory with checkpoint*)
+(*checks N first, then N'*)
+Definition updatemaps (N: nvmem) (N': nvmem): nvmem :=
+  match N, N' with
+    NonVol m D, NonVol m' D' => NonVol
+  (fun j =>
+     match m j with
+     error => m' j
+     | x => x
+     end
+  )
+  (D ++ D') (*inclusion of duplicates*)
+  end.
+Notation "m1 'U!' m2" := (updatemaps m1 m2) (at level 100).
+(*start here should really change the above ordering to be more intuitive*)
+
+Notation emptyNV := (NonVol (emptymap loc_eqtype) nil).
+Definition reset (V: vmem) := Vol (emptymap loc_eqtype).
+
+(*restricts memory map m to domain w*)
+(*doesn't actually clean the unnecessary variables out of m*)
+(*need a decidable In here*)
+Lemma decidable_loc: forall(x y: loc), {x = y} + {x <> y}.
+  intros. destruct (x == y) eqn: beq.
+  apply left. apply: eqP beq.
+  apply right. apply (elimF eqP beq).
+Qed.
+(*start here how to use the reflect/move stuff when things
+ are false*)
+Lemma decidable_in: forall(x: loc) (w: warvars),
+    {In x w} + {not (In x w)}.
+apply (in_dec decidable_loc). Qed.
+
+
+(*removes L1 from L2 *)
+Definition remove (L1 L2 : list loc) :=
+  filter (fun x =>  sumbool_not _ _ (decidable_in x L1)
+            ) L2.
+
+Definition restrict (N: nvmem) (w: warvars): nvmem :=
+  match N with NonVol m D => NonVol
+    (fun input => if (decidable_in input w) then m input else error) w  end.
+
+Notation "N '|!' w" := (restrict N w) 
+  (at level 40, left associativity).
+
+(*prop determining if every location in array a is in the domain of m*)
+Definition indomain_nvm (N: nvmem) (w: loc) :=
+  In w (getdomain N).
+
+(*equality type for list loc*)
+
+Fixpoint eqb_warvars (w1: warvars) (w2: warvars) :=
+  match w1, w2 with
+    [], [] => true
+  | (x::xs), (y::ys) => (x == y) && (eqb_warvars xs ys)
+  | _, _ => false 
+  end.
+
+Lemma eqb_wv_refl: forall y: warvars, is_true (eqb_warvars y y).
+  Admitted.
+
+Lemma eqb_wv_true_iff : forall x y : warvars,
+    is_true(eqb_warvars x y) <-> x = y.
+Proof.
+  intros. induction x.
+  + split. destruct y. simpl. auto.
+    unfold eqb_warvars. simpl. intros contra. discriminate contra.
+    move ->. Admitted.
+
+Lemma eqwv: Equality.axiom eqb_warvars.
+Proof.
+Admitted.
+
+Canonical wv_eqMixin := EqMixin eqwv.
+Canonical wv_eqtype := Eval hnf in EqType warvars wv_eqMixin.
+
+Definition isdomain_nvm (N: nvmem) (w: warvars) :=
+  (getdomain N) == w.
+Definition subset_nvm (N1 N2: nvmem) :=
+  (incl (getdomain N1) (getdomain N2)) /\ (forall(l: loc),
+                                    In l (getdomain N1) ->
+                                    (getmap N1) l = (getmap N2) l
+                                  ).
+(********************************************)
+Inductive cconf := (*continuous configuration*)
+  ContinuousConf (triple: nvmem * vmem * command).
+
+Notation context := (nvmem * vmem * command).
+
+(*A coercion for cconf doesn't work because it's the same essential type as context.
+ So, in practice, to avoid writing the constructor everywhere, I've been using contexts foralleverything, when conceptually a cconf would make more sense.
+ It would be nice to just have one type for this.*)
+
+Notation iconf := (context * nvmem * vmem * command).
+
+Definition getcom (C: context) :=
+  match C with
+    (_, _, out) => out end.
+
+Definition ro := loc * value. (*read observation*)
+Definition readobs := list ro.
+
+Notation NoObs := ([]: readobs).
+
+Inductive obs := (*observation*)
+  Obs (r: readobs)
+| reboot
+| checkpoint.
+Coercion Obs : readobs >-> obs.
+
+Notation obseq := (list obs). (*observation sequence*)
+
+Open Scope list_scope.
+
+(*helpers for configs*)
+Inductive single_com: context -> Prop :=
+  SingleCom: forall(N: nvmem) (V: vmem) (l: instruction),
+               single_com (N, V, Ins l).
+
+Definition single_com_i (C: iconf) :=
+  match C with (_, _, c) =>
+  (match c with
+    Ins _ => True
+  | _ => False end) end.
+
+(*helpers for observations and warvars*)
+
+(*converts from list of read locations to list of
+WAR variables
  *)
-(*took out equality premises and built them into the types*)
-Check same_pt.
-Inductive same_config: iconf -> context -> Prop :=
-  SameConfig: forall(N0 N1 N2: nvmem)
-                (V0 V: vmem)
-                (c0 c: command),
-                same_pt N0 V0 c0 c N1 N2 -> (*nvms are extensionally the same by same_pt
-                                          vms and cs are intensionally the same by types*)
-                same_config ((N0, V0, c0), N1, V, c) (N2, V, c).
 
+Fixpoint readobs_loc (R: readobs): (list loc) := 
+  match R with
+    nil => nil
+| (r::rs) => match r with
+             (location, _) => location :: (readobs_loc rs)
+           end
+  end.
+
+
+(*relations between continuous and intermittent observations*)
+(*Definition reduces (O1 O2: readobs) :=
+  (prefix O1 O2*)
+Notation "S <= T" := (prefix S T).
+
+(*Where
+O1 is a sequence of read observation lists,
+where each continguous read observation list is separated from those adjacent to it by a reboot,
+and O2 is a read observation list,
+prefix_seq determines if each ro list in O1 is a valid
+prefix of O2*)
+Inductive prefix_seq: obseq -> readobs -> Prop :=
+  RB_Base: forall(O: readobs), prefix_seq [Obs O] O
+| RB_Ind: forall(O1 O2: readobs) (O1': obseq),
+    O1 <= O2 -> prefix_seq O1' O2 -> prefix_seq ([Obs O1] ++ [reboot] ++ O1') O2.
+
+(* Where
+O1 is a sequence of ((read observation list sequences), where
+each continguous read observation list is separated from those adjacent to it
+by a reboot), where each sequence is separated from those adjacent to it by a checkpoint.
+ie, each read observation list in a given read observation sequence
+occurs within the same checkpointed region as all the other read observation lists in that sequence,
+O2 is a read observation list,
+prefix_frag determines if each ro list in O1 is a prefix of some FRAGMENT of O2
+(where the fragments are separated by the positioning of the checkpoints in O1)
+ *)
+Inductive prefix_fragment: obseq -> readobs -> Prop :=
+  CP_Base: forall(O1: obseq) (O2: readobs), prefix_seq O1 O2 -> prefix_fragment O1 O2
+| CP_IND: forall(O1 O1': obseq) (O2 O2': readobs),
+    prefix_seq O1 O2 -> prefix_fragment O1' O2' ->
+   prefix_fragment (O1 ++ [checkpoint] ++ O1') (O2 ++ O2'). 
+
+(***************************************************************)
+
+
+(****************continuous operational semantics***********************)
+(*evaluation relation for expressions*)
+
+Inductive eeval: nvmem -> vmem -> exp -> readobs -> value -> Prop :=
+  VAL: forall(N: nvmem) (V: vmem) (v: value),
+    (isvaluable v) -> (*extra premise to check if v is valuable*)
+    eeval N V v NoObs v
+| BINOP: forall(N: nvmem) (V: vmem)
+          (e1: exp) (e2: exp)
+          (r1: readobs) (r2: readobs)
+          (v1: value) (v2: value) (bop: boptype),
+    eeval N V e1 r1 v1 ->
+    eeval N V e2 r2 v2 -> 
+    (isvalidbop bop v1 v2) -> (*extra premise to check if v1, v2, bop v1 v2 valuable*)
+    eeval N V (Bop bop e1 e2) (r1++ r2) (bopeval bop v1 v2)
+| RD_VAR_NV: forall(N: nvmem) (mapV: vmem) (x: smallvar) (v: value),
+    ((inl x) <-N) = v ->
+    isNV(x) -> (*extra premise to make sure x is correct type for NV memory*)
+    (isvaluable v) -> (*extra premise to check if v is valuable*)
+    eeval N mapV x [((inl x), v)] v
+| RD_VAR_V: forall(N: nvmem) (mapV: mem) (x: smallvar) (v: value),
+    (mapV (inl x)) = v ->
+    isV(x) -> (*extra premise to make sure x is correct type for V memory*)
+    (isvaluable v) -> (*extra premise to check if v is valuable*)
+    eeval N (Vol mapV) x [((inl x), v)] v
+| RD_ARR: forall(N: nvmem) (V: vmem)
+           (a: array)
+           (index: exp)
+           (rindex: readobs)
+           (vindex: value)
+           (element: el)
+           (v: value),
+    eeval N V (index) rindex vindex ->
+    ((inr element) <-N) = v ->
+    (val element) = (El_d a vindex) -> (*extra premise to check that inr element
+                                        is actually a[vindex] *)
+(*well-typedness, valuability, inboundedness of vindex are checked in elpred*)
+    (isvaluable v) -> (*extra premise to check if v is valuable*)
+    eeval N V (a[[index]]) (rindex++[((inr element), v)]) v
+.
+
+(****************************************************************************)
+
+(**********continuous execution semantics*************************)
+
+
+(*evaluation relation for commands*)
+
+
+
+(*written, read, written before reading*)
+Notation the_write_stuff := ((list loc) * (list loc) * (list loc)).
+
+(*consider using a record type so I don't need so many of these*)
+
+Definition getwt (W: the_write_stuff) := match W with (out, _, _ )=> out end.
+
+Definition getrd (W: the_write_stuff) := match W with (_, out , _ )=> out end.
+
+Definition getfstwt (W: the_write_stuff) := match W with (_, _, out )=> out end.
+
+Notation emptysets := ((nil : (list loc)), (nil: (list loc)), (nil: (list loc))).
+
+
+
+(***Below, I define an evaluation relation for continuous programs which accumulates
+ read/write data as the program evaluates. This makes the trace type more elegant, while
+ also containing the same data as the cceval above.
+However, the write data does not influence the evaluation of the program, so, if it were not
+for the trace type, it wouldn't be clear I would include this here.
+It not included in the evaluation relation in the paper.
+ **)
+(*Single steps, accumulates write data*)
+(*Note: program consisting of just a checkpoint is illegal...huh*)
+
+Inductive cceval_w: context -> obseq -> context -> the_write_stuff -> Prop :=
+CheckPoint: forall(N: nvmem)
+               (V: vmem)
+               (c: command)
+               (w: warvars),
+    cceval_w (N, V, ((incheckpoint w);; c))
+             [checkpoint]
+             (N, V, c)
+             (nil, nil, nil)
+| NV_Assign: forall(x: smallvar) (N: nvmem) (V: vmem) (e: exp) (r: readobs) (v: value),
+    eeval N V e r v ->
+    isNV(x) -> (*checks x is correct type for NV memory*)
+    (isvaluable v) -> (*extra premise to check if v is valuable*)
+    cceval_w (N, V, Ins (asgn_sv x e))
+             [Obs r]
+             ((updateNV N (inl x) v), V, Ins skip)
+             ([inl x],  (readobs_loc r), (remove (readobs_loc r) [inl x]))
+| V_Assign: forall(x: smallvar) (N: nvmem) (mapV: mem) (e: exp) (r: readobs) (v: value),
+    eeval N (Vol mapV) e r v ->
+    isV(x) -> (*checks x is correct type for V memory*)
+    (isvaluable v) -> (*extra premise to check if v is valuable*)
+    cceval_w (N, (Vol mapV), Ins (asgn_sv x e)) [Obs r]
+             (N, (Vol ((inl x) |-> v ; mapV)), Ins skip)
+             (nil,  (readobs_loc r), nil)
+| Assign_Arr: forall (N: nvmem) (V: vmem)
+               (a: array)
+               (ei: exp)
+               (ri: readobs)
+               (vi: value)
+               (e: exp)
+               (r: readobs)
+               (v: value)
+               (element: el),
+    eeval N V ei ri vi ->
+    eeval N V e r v ->
+    (val element) = (El_d a vi) -> (*extra premise to check that inr element
+                                        is actually a[vindex] *)
+(*well-typedness, valuability, inboundedness of vindex are checked in elpred*)
+    (isvaluable v) -> (*extra premise to check if v is valuable*)
+    cceval_w (N, V, Ins (asgn_arr a ei e))
+           [Obs (ri++r)]
+           ((updateNV N (inr element) v), V, Ins skip)
+           ([inr element], (readobs_loc (ri ++ r)), (remove (readobs_loc (ri ++ r)) [inr element]))
+(*valuability and inboundedness of vindex are checked in sameindex*)
+| Skip: forall(N: nvmem)
+         (V: vmem)
+         (c: command),
+    cceval_w (N, V, (skip;;c)) [Obs NoObs] (N, V, c) (nil, nil, nil)
+| Seq: forall (N N': nvmem)
+         (V V': vmem)
+         (l: instruction)
+         (c: command)
+         (o: obs)
+         (W: the_write_stuff),
+    (forall(w: warvars), l <> (incheckpoint w)) ->
+    l <> skip ->
+    cceval_w (N, V, Ins l) [o] (N', V', Ins skip) W ->
+    cceval_w (N, V, (l;;c)) [o] (N', V', c) W
+   (*IP becomes obnoxious if you let checkpoint into the Seq case so I'm outlawing it
+    same with skip*) 
+| If_T: forall(N: nvmem)
+         (V: vmem)
+         (e: exp)
+         (r: readobs)
+         (c1 c2: command),
+    eeval N V e r true -> (*yuh doy not writing anything in eeval*)
+    cceval_w (N, V, (TEST e THEN c1 ELSE c2)) [Obs r] (N, V, c1) (nil, (readobs_loc r), nil)
+| If_F: forall(N: nvmem)
+         (V: vmem)
+         (e: exp)
+         (r: readobs)
+         (c1 c2: command),
+    eeval N V e r false ->
+    cceval_w (N, V, (TEST e THEN c1 ELSE c2)) [Obs r] (N, V, c2) (nil, (readobs_loc r), nil).
+
+Definition append_write (W1 W2: the_write_stuff) :=
+  ((getwt W1) ++ (getwt W2), (getrd W1) ++ (getrd W2), (getfstwt W1) ++ (remove (getrd W1) (getfstwt W2))).
+(************************************************************)
+
+(**********intermittent execution semantics*************************)
+(*evaluation relation for commands*)
+(*accumlates write data as continuous relation does*)
+Inductive iceval_w: iconf -> obseq -> iconf -> the_write_stuff -> Prop :=
+  CP_PowerFail: forall(k: context) (N: nvmem) (V: vmem) (c: command),
+                 iceval_w (k, N, V, c)
+                        nil
+                        (k, N, (reset V), Ins inreboot) (nil, nil, nil)
+ | CP_Reboot: forall(N N': nvmem) (*see below*) (*N is the checkpointed one*)
+               (V V': vmem) 
+               (c: command), 
+     iceval_w ((N, V, c), N', V', Ins inreboot)
+            [reboot]
+            ((N, V, c), (N U! N'), V, c) (nil, nil, nil)
+ | CP_CheckPoint: forall(k: context) (N: nvmem) (V: vmem) (c: command) (w: warvars),
+                 iceval_w (k, N, V, ((incheckpoint w);;c))
+                        [checkpoint]
+                        (((N |! w), V, c), N, V, c) (nil, nil, nil) 
+ | CP_NV_Assign: forall(k: context) (x: smallvar) (N: nvmem) (V: vmem) (e: exp) (r: readobs) (v: value),
+    eeval N V e r v ->
+    isNV(x) -> (*checks x is correct type for NV memory*)
+    (isvaluable v) -> (*extra premise to check if v is valuable*)
+    iceval_w (k, N, V, Ins (asgn_sv x e))
+           [Obs r]
+           (k, (updateNV N (inl x) v), V, Ins skip)
+           ([inl x],  (readobs_loc r), (remove (readobs_loc r) [inl x]))
+| CP_V_Assign: forall(k: context) (x: smallvar) (N: nvmem) (mapV: mem) (e: exp) (r: readobs) (v: value),
+    eeval N (Vol mapV) e r v ->
+    isV(x) -> (*checks x is correct type for V memory*)
+    (isvaluable v) -> (*extra premise to check if v is valuable*)
+    iceval_w (k, N, (Vol mapV), Ins (asgn_sv x e))
+           [Obs r]
+           (k, N, (Vol ((inl x) |-> v ; mapV)), Ins skip)
+             (nil,  (readobs_loc r), nil)
+| CP_Assign_Arr: forall (k: context) (N: nvmem) (V: vmem)
+               (a: array)
+               (ei: exp)
+               (ri: readobs)
+               (vi: value)
+               (e: exp)
+               (r: readobs)
+               (v: value)
+               (element: el),
+    eeval N V ei ri vi ->
+    eeval N V e r v ->
+    (val element) = (El_d a vi) -> (*extra premise to check that inr element                                        is actually a[vi] *)
+(*well-typedness, valuability, inboundedness of vindex are checked in elpred*)
+    (isvaluable v) -> (*extra premise to check if v is valuable*)
+    iceval_w (k, N, V, Ins (asgn_arr a ei e))
+           [Obs (ri++r)]
+           (k, (updateNV N (inr element) v), V, Ins skip)
+           ([inr element], (readobs_loc (ri ++ r)), (remove  (readobs_loc (ri ++ r)) [inr element]))
+| CP_Skip: forall(k: context) (N: nvmem)
+         (V: vmem)
+         (c: command),
+    iceval_w (k, N, V, (skip;;c)) [Obs NoObs] (k, N, V, c) (nil, nil, nil)
+|CP_Seq: forall (k: context)
+         (N: nvmem) (N': nvmem)
+         (V: vmem) (V': vmem)
+         (l: instruction)
+         (c: command)
+         (o: obs)
+         (W: the_write_stuff),
+    iceval_w (k, N, V, Ins l) [o] (k, N', V', Ins skip) W ->
+    iceval_w (k, N, V, (l;;c)) [o] (k, N', V', c) W
+|CP_If_T: forall(k: context) (N: nvmem) (V: vmem)
+         (e: exp)
+         (r: readobs)
+         (c1 c2: command),
+    eeval N V e r true -> 
+    iceval_w (k, N, V, (TEST e THEN c1 ELSE c2)) [Obs r] (k, N, V, c1) (nil, (readobs_loc r), nil)
+|CP_If_F: forall(k: context) (N: nvmem) (V: vmem)
+         (e: exp)
+         (r: readobs)
+         (c1 c2: command),
+    eeval N V e r false ->
+    iceval_w (k, N, V, (TEST e THEN c1 ELSE c2)) [Obs r] (k, N, V, c2) (nil, (readobs_loc r), nil).
+(*CP_Reboot: I took out the equals premise and instead built it
+into the types because I didn't want to define a context equality function*)
+
+(********************************************)
+(*helpers that use the evals
+Definition el_arrayexp_eq (e: el) (a: array) (eindex: exp) (N: nvmem) (V: vmem) := (*transitions from el type to a[exp] representation*)
+  (samearray e a) /\
+  exists(r: readobs) (vindex: value), eeval N V eindex r vindex /\
+                                 (eq_value (getindexel e) vindex).*)
+(******)
 Close Scope list_scope.
 Close Scope type_scope.
